src/protocol/DNS.Protocol.Parser.EverParseAdapter.fst
@@ -100,10 +100,12 @@ let generated_dns_uncompressed_question_mx_answer_packet_validator
     exchange_name_length
 
 let generated_dns_uncompressed_question_compressed_mx_answer_packet_validator
-    qname_length rr_name_length =
+    qname_length rr_name_length exchange_name_ptr_hi_value exchange_name_ptr_lo_value =
   DNSProtocol.validate__dns_uncompressed_question_compressed_mx_answer_packet
     qname_length
     rr_name_length
+    exchange_name_ptr_hi_value
+    exchange_name_ptr_lo_value
 
 let generated_dns_uncompressed_question_soa_answer_packet_validator
     qname_length rr_name_length mname_length rname_length =
